{
 "cells": [
  {
   "cell_type": "markdown",
   "metadata": {},
   "source": [
    "## Problem 1"
   ]
  },
  {
   "cell_type": "markdown",
   "metadata": {},
   "source": [
    "# a)\n",
    "\n",
    "We want to obtain log-likelihood function for a random sample of n observations. Our likelihood function looks like this:\n",
    "\n",
    "\\begin{equation*}\n",
    "L(\\alpha, \\beta | x ) = \\Pi_{i=1}^n f(x_i | \\alpha , \\beta )\n",
    "\\end{equation*}\n",
    "\n",
    "Now we logarithmize both sides of likelihood function and perform several computations in order to simplify result:\n",
    "\n",
    "\\begin{equation*}\n",
    "\\ln L(\\alpha, \\beta | x ) = \\sum_{i=1}^n \\ln f(x_i | \\alpha , \\beta ) = \n",
    "\\sum_{i=1}^n \\ln (\\alpha \\beta x_{i}^{\\beta-1}e^{-\\alpha x_i^\\beta}) = \n",
    "\\sum_{i=1}^n \\Big( \\ln(\\alpha \\beta) + (\\beta-1) \\ln(x_i)-\\alpha x_i^\\beta \\Big) = \n",
    "n \\ln (\\alpha \\beta ) + (\\beta - 1) \\sum_{i=1}^n \\Big(\\ln(x_i)\\Big) - \\alpha \\sum_{i=1}^n x_i^\\beta\n",
    "\\end{equation*}\n",
    "\n",
    "\n",
    "Our log-likelihood function for a random sample of n observations:\n",
    "\\begin{equation*}\n",
    "\\ln L(\\alpha, \\beta | x ) = n \\ln (\\alpha \\beta ) + (\\beta - 1) \\sum_{i=1}^n (\\ln(x_i)) - \\alpha \\sum_{i=1}^n x_i^\\beta\n",
    "\\end{equation*}"
   ]
  },
  {
   "cell_type": "markdown",
   "metadata": {},
   "source": [
    "# b)\n",
    "\n",
    "Necessary condition equations for $\\alpha$ and $\\beta$ can be easily derived by taking first derivatives of the log-likelihood function with respect to $\\alpha$ and $\\beta$ respectively and setting them to be equal to zero:\\\n",
    "(This makes sense, as we are trying to maximize the log-likelihood function) \n",
    "\n",
    "\n",
    "$$\n",
    "\\left[\\begin{array}{cc} \n",
    "\\frac{\\partial \\ln L}{\\partial \\alpha} \\\\\n",
    "\\frac{\\partial \\ln L}{\\partial \\beta}\n",
    "\\end{array}\\right] =\n",
    "\\left[\\begin{array}{cc} \n",
    "\\frac{n}{\\alpha} - \\sum_{i=1}^n x_i^\\beta \\\\ \n",
    "\\frac{n}{\\beta} + \\sum_{i=1}^n \\Big( \\ln ( x_i ) \\Big) - \\alpha \\ln (\\beta) \\sum_{i=1}^n x_i^\\beta\n",
    "\\end{array}\\right] =\n",
    "\\left[\\begin{array}{cc} \n",
    "0 \\\\ \n",
    "0\n",
    "\\end{array}\\right]\n",
    "$$\n",
    "\n",
    "\n",
    "From this we can easily derive that $\\alpha = \\frac{n}{\\sum_{i=1}^n x_i^\\beta}$. In order to obtain maximizing value of $\\beta$ we need to plug into second equation vlaue of $\\alpha$:\n",
    "\n",
    "\n",
    "\\begin{equation*}\n",
    "0 = \\frac{n}{\\beta} + \\sum_{i=1}^n \\Big( \\ln ( x_i ) \\Big) - \\alpha \\ln (\\beta) \\sum_{i=1}^n x_i^\\beta = \n",
    "\\frac{n}{\\beta} + \\sum_{i=1}^n \\Big( \\ln ( x_i ) \\Big) - \\frac{n}{\\sum_{i=1}^n x_i^\\beta} \\ln (\\beta) \\sum_{i=1}^n x_i^\\beta =\n",
    "\\frac{n}{\\beta}-n \\ln (\\beta)\n",
    "\\end{equation*}\n",
    "\n",
    "\\begin{equation*}\n",
    "0 = \\frac{n}{\\beta}-n \\ln (\\beta)\n",
    "\\end{equation*}\n",
    "\n",
    "\\begin{equation*}\n",
    "\\beta \\ ln \\beta = 1\n",
    "\\end{equation*}\n",
    "\n",
    "\n",
    "This is hardly \"nice\" solution. To obtain value of $\\beta$ as a real number, we need to apply Lambert W function:\n",
    "\n",
    "\\begin{equation*}\n",
    "\\beta \\ ln \\beta = 1\n",
    "\\end{equation*}\n",
    "\n",
    "\\begin{equation*}\n",
    "e^{ \\ln \\beta} \\ ln \\beta = 1\n",
    "\\end{equation*}\n",
    "\n",
    "\\begin{equation*}\n",
    "\\ln \\beta = W(1)\n",
    "\\end{equation*}\n",
    "\n",
    "\\begin{equation*}\n",
    "\\beta = e^W(1)\n",
    "\\end{equation*}\n",
    "\n",
    "\n",
    "\n",
    "\n",
    "\n"
   ]
  }
 ],
 "metadata": {
  "kernelspec": {
   "display_name": "R",
   "language": "R",
   "name": "ir"
  },
  "language_info": {
   "codemirror_mode": "r",
   "file_extension": ".r",
   "mimetype": "text/x-r-source",
   "name": "R",
   "pygments_lexer": "r",
   "version": "3.6.1"
  }
 },
 "nbformat": 4,
 "nbformat_minor": 4
}
